Address state_rel problem with code_includes
This commit removes the problematic code_includes from state_rel and
instead pushes the current code table through v_rel and friends. This
way, if there is an optimised closure value, then its corresponding
code is part of the current code table. This approach gets around the
problem, but makes the proofs a bit more ugly.

There are several cheats in this commit. Most of them are routine
cases (If, Handle, Raise) that have yet to be updated for the new
v_rel. There are also some simple theorems about v_rel that are
cheated. These simple cheats are marked with comments "routine proof".

compiler/backend/proofs/clos_callProofScript.sml
@@ -169,8 +169,12 @@ val recclosure_wf_def = Define`
     DISJOINT (set (GENLIST (λi. 2 * i + loc) (LENGTH fns))) (set (code_locs (MAP SND fns))) ∧
     ALL_DISTINCT (code_locs (MAP SND fns))`;
 
+val code_includes_def = Define`
+  code_includes al code ⇔
+    ∀k v. ALOOKUP al k = SOME v ⇒ FLOOKUP code k = SOME v`;
+
 val recclosure_rel_def = Define`
-  recclosure_rel g l loc fns1 fns2 ⇔ ∃g0.
+  recclosure_rel g l code loc fns1 fns2 ⇔ ∃g0.
      recclosure_wf loc fns1 ∧
      wfg g0 ∧
      DISJOINT (IMAGE SUC (set (code_locs (MAP SND fns1)))) (set (MAP FST (SND g0))) ∧
@@ -180,13 +184,15 @@ val recclosure_rel_def = Define`
      then
        (∃tra n. fns2 = calls_list tra n loc fns1) ∧
        subg (code_list loc (ZIP (MAP FST fns1,es)) new_g) g ∧
-       set (code_locs (MAP SND fns1)) DIFF domain (FST new_g) ⊆ l
+       set (code_locs (MAP SND fns1)) DIFF domain (FST new_g) ⊆ l ∧
+       code_includes (SND (code_list loc (ZIP (MAP FST fns1,es)) new_g)) code
      else
        let (es,new_g) = calls (MAP SND fns1) g0 in
        fns2 = ZIP (MAP FST fns1, es) ∧
        subg new_g g ∧
        set (code_locs (MAP SND fns1)) DIFF domain (FST new_g) ⊆ l ∧
-       set (GENLIST (λi. 2*i+loc) (LENGTH fns1)) ⊆ l`;
+       set (GENLIST (λi. 2*i+loc) (LENGTH fns1)) ⊆ l ∧
+       code_includes (SND new_g) code`;
 
 val env_rel_def = Define`
   env_rel R env1 env2 a es ⇔
@@ -207,57 +213,54 @@ val env_rel_cong = Q.store_thm("env_rel_cong[defncong]",
   rw[env_rel_def,MEM_EL,PULL_EXISTS,EQ_IMP_THM,LIST_REL_EL_EQN]);
 
 val v_rel_def = tDefine"v_rel"`
-  (v_rel g l (Number i) v ⇔ v = Number i) ∧
-  (v_rel g l (Word64 w) v ⇔ v = Word64 w) ∧
-  (v_rel g l (Block n vs) v ⇔
-    ∃vs'. v = Block n vs' ∧ LIST_REL (v_rel g l) vs vs') ∧
-  (v_rel g l (ByteVector ws) v ⇔ v = ByteVector ws) ∧
-  (v_rel g l (RefPtr n) v ⇔ v = RefPtr n) ∧
-  (v_rel g l (Closure loco vs1 env1 n bod1) v ⇔
+  (v_rel g l code (Number i) v ⇔ v = Number i) ∧
+  (v_rel g l code (Word64 w) v ⇔ v = Word64 w) ∧
+  (v_rel g l code (Block n vs) v ⇔
+    ∃vs'. v = Block n vs' ∧ LIST_REL (v_rel g l code) vs vs') ∧
+  (v_rel g l code (ByteVector ws) v ⇔ v = ByteVector ws) ∧
+  (v_rel g l code (RefPtr n) v ⇔ v = RefPtr n) ∧
+  (v_rel g l code (Closure loco vs1 env1 n bod1) v ⇔
      ∃loc vs2 env2 bod2.
-       recclosure_rel g l loc [(n,bod1)] [(n,bod2)] ∧
+       recclosure_rel g l code loc [(n,bod1)] [(n,bod2)] ∧
        v = Closure (SOME loc) vs2 env2 n bod2 ∧ loco = SOME loc ∧
-       LIST_REL (v_rel g l) vs1 vs2 ∧
-       env_rel (v_rel g l) env1 env2 0 [(n,bod2)]) ∧
-  (v_rel g l (Recclosure loco vs1 env1 fns1 i) v ⇔
+       LIST_REL (v_rel g l code) vs1 vs2 ∧
+       env_rel (v_rel g l code) env1 env2 0 [(n,bod2)]) ∧
+  (v_rel g l code (Recclosure loco vs1 env1 fns1 i) v ⇔
      ∃loc vs2 env2 fns2.
-       recclosure_rel g l loc fns1 fns2 ∧
+       recclosure_rel g l code loc fns1 fns2 ∧
        v = Recclosure (SOME loc) vs2 env2 fns2 i ∧ loco = SOME loc ∧
-       LIST_REL (v_rel g l) vs1 vs2 ∧
-       env_rel (v_rel g l) env1 env2 (LENGTH fns2) fns2)`
-  (WF_REL_TAC `measure (v_size o FST o SND o SND)` >> simp[v_size_def] >>
+       LIST_REL (v_rel g l code) vs1 vs2 ∧
+       env_rel (v_rel g l code) env1 env2 (LENGTH fns2) fns2)`
+  (WF_REL_TAC `measure (v_size o FST o SND o SND o SND)` >> simp[v_size_def] >>
    rpt strip_tac >> imp_res_tac v_size_lemma >> simp[]);
 
 val v_rel_ind = theorem"v_rel_ind";
 
-val code_includes_def = Define`
-  code_includes al code ⇔
-    ∀k v. ALOOKUP al k = SOME v ⇒ FLOOKUP code k = SOME v`;
-
 val wfv_def = tDefine"wfv"`
-  (wfv g l (Closure NONE _ _ _ _) ⇔ F) ∧
-  (wfv g l (Recclosure NONE _ _ _ _) ⇔ F) ∧
-  (wfv g l (Closure (SOME loc) vs env n bod) ⇔
-    EVERY (wfv g l) vs ∧ EVERY (wfv g l) env ∧
+  (wfv g l code (Closure NONE _ _ _ _) ⇔ F) ∧
+  (wfv g l code (Recclosure NONE _ _ _ _) ⇔ F) ∧
+  (wfv g l code (Closure (SOME loc) vs env n bod) ⇔
+    EVERY (wfv g l code) vs ∧ EVERY (wfv g l code) env ∧
     ∃fns2.
-    recclosure_rel g l loc [(n,bod)] fns2) ∧
-  (wfv g l (Recclosure (SOME loc) vs env fns i) ⇔
-    EVERY (wfv g l) vs ∧ EVERY (wfv g l) env ∧
+    recclosure_rel g l code loc [(n,bod)] fns2) ∧
+  (wfv g l code (Recclosure (SOME loc) vs env fns i) ⇔
+    EVERY (wfv g l code) vs ∧ EVERY (wfv g l code) env ∧
     ∃fns2.
-    recclosure_rel g l loc fns fns2) ∧
-  (wfv g l (Block _ vs) ⇔ EVERY (wfv g l) vs) ∧
-  (wfv _ _ _ ⇔ T)`
-  (WF_REL_TAC `measure (v_size o SND o SND)` >> simp[v_size_def] >>
+    recclosure_rel g l code loc fns fns2) ∧
+  (wfv g l code (Block _ vs) ⇔ EVERY (wfv g l code) vs) ∧
+  (wfv _ _ _ _ ⇔ T)`
+  (WF_REL_TAC `measure (v_size o SND o SND o SND)` >> simp[v_size_def] >>
    rpt strip_tac >> imp_res_tac v_size_lemma >> simp[]);
 val _ = export_rewrites["wfv_def"];
 
 val wfv_ind = theorem"wfv_ind";
 
 val wfv_state_def = Define`
-  wfv_state g l s ⇔
-    EVERY (OPTION_EVERY (wfv g l)) s.globals ∧
-    FEVERY (every_refv (wfv g l) o SND) s.refs ∧
-    s.code = FEMPTY ∧ !k. SND (SND (s.compile_oracle k)) = []`;
+  wfv_state g l code s ⇔
+    EVERY (OPTION_EVERY (wfv g l code)) s.globals ∧
+    FEVERY (every_refv (wfv g l code) o SND) s.refs ∧
+    s.code = FEMPTY ∧
+    !k. SND (SND (s.compile_oracle k)) = [] (* TODO: remove this line *)`;
 
 val _ = temp_type_abbrev("calls_state",
           ``:num_set # (num, num # closLang$exp) alist``);
@@ -267,8 +270,8 @@ val state_rel_def = Define`
     (s.ffi = t.ffi) ∧
     (s.clock = t.clock) ∧
     (s.max_app = t.max_app) ∧
-    LIST_REL (OPTREL (v_rel g l)) s.globals t.globals ∧
-    fmap_rel (ref_rel (v_rel g l)) s.refs t.refs ∧
+    LIST_REL (OPTREL (v_rel g l t.code)) s.globals t.globals ∧
+    fmap_rel (ref_rel (v_rel g l t.code)) s.refs t.refs ∧
     s.code = FEMPTY (* ∧ code_includes (SND g) t.code *)`;
 
 val state_rel_max_app = Q.store_thm("state_rel_max_app",
@@ -285,7 +288,7 @@ val state_rel_with_clock = Q.store_thm("state_rel_with_clock",
 
 val state_rel_flookup_refs = Q.store_thm("state_rel_flookup_refs",
   `state_rel g l s t ∧ FLOOKUP s.refs k = SOME v ⇒
-   ∃v'. FLOOKUP t.refs k = SOME v' ∧ ref_rel (v_rel g l) v v'`,
+   ∃v'. FLOOKUP t.refs k = SOME v' ∧ ref_rel (v_rel g l t.code) v v'`,
   rw[state_rel_def,fmap_rel_OPTREL_FLOOKUP]
   \\ first_x_assum(qspec_then`k`mp_tac) \\ rw[OPTREL_def]);
 
@@ -871,7 +874,7 @@ val calls_el_sing = Q.store_thm("calls_el_sing",
 (* properties of value relation *)
 
 val v_rel_exists = Q.store_thm("v_rel_exists",
-  `∀v1. wfv g l v1 ⇒ ∃v2. v_rel g l v1 v2`,
+  `∀v1. wfv g l code v1 ⇒ ∃v2. v_rel g l code v1 v2`,
   ho_match_mp_tac v_ind
   \\ rw[v_rel_def]
   >- (
@@ -903,16 +906,16 @@ val v_rel_exists = Q.store_thm("v_rel_exists",
     \\ metis_tac[SKOLEM_THM] ));
 
 val v_rel_subg = Q.store_thm("v_rel_subg",
-  `∀g l v1 v2 g' l'.
-    v_rel g l v1 v2 ∧ subg g g' ∧ l ⊆ l' ⇒
-    v_rel g' l' v1 v2`,
+  `∀g l code v1 v2 g' l'.
+    v_rel g l code v1 v2 ∧ subg g g' ∧ l ⊆ l' ⇒
+    v_rel g' l' code v1 v2`,
   ho_match_mp_tac v_rel_ind
   \\ rw[v_rel_def,env_rel_def,recclosure_rel_def]
   \\ Cases_on`LENGTH env1 = LENGTH env2`
   \\ fsrw_tac[ETA_ss][PULL_FORALL,PULL_EXISTS]
   \\ rpt(
-    qmatch_assum_abbrev_tac`LIST_REL (v_rel g l) l1 l2`
-    \\ `LIST_REL (v_rel g' l') l1 l2`
+    qmatch_assum_abbrev_tac`LIST_REL (v_rel g l code) l1 l2`
+    \\ `LIST_REL (v_rel g' l' code) l1 l2`
     by (
       match_mp_tac EVERY2_MEM_MONO
       \\ first_assum(part_match_exists_tac (last o strip_conj) o concl)
@@ -920,7 +923,7 @@ val v_rel_subg = Q.store_thm("v_rel_subg",
       \\ imp_res_tac LIST_REL_LENGTH
       \\ simp[MEM_ZIP,PULL_EXISTS]
       \\ metis_tac[MEM_EL] )
-    \\ qpat_x_assum`LIST_REL (v_rel g l) l1 l2` kall_tac
+    \\ qpat_x_assum`LIST_REL (v_rel g l code) l1 l2` kall_tac
     \\ map_every qunabbrev_tac[`l2`,`l1`])
   \\ fs[]
   \\ qexists_tac`g0`
@@ -966,8 +969,8 @@ val code_includes_ALOOKUP = Q.store_thm("code_includes_ALOOKUP",
 
 val dest_closure_v_rel_lookup = Q.store_thm("dest_closure_v_rel_lookup",
   `dest_closure max_app (SOME loc) v1 env1 = SOME x ∧
-   v_rel g l v1 v2 ∧
-   LIST_REL (v_rel g l) env1 env2 ∧
+   v_rel g l code v1 v2 ∧
+   LIST_REL (v_rel g l code) env1 env2 ∧
    wfg g ∧ loc ∈ domain (FST g) ∧ loc ∉ l  ⇒
    ∃e l1 xs n ls g01 g1 l1' tra i.
      x = Full_app e (env1++l1) [] ∧ EL n xs = (LENGTH env1,e) ∧
@@ -975,7 +978,9 @@ val dest_closure_v_rel_lookup = Q.store_thm("dest_closure_v_rel_lookup",
      subg (code_list (loc - 2*n) (ZIP (MAP FST xs,ls)) g1) g ∧
      ALOOKUP (SND g) (loc+1) = SOME (LENGTH env1,EL n ls) ∧
      dest_closure max_app (SOME loc) v2 env2 =
-       SOME (Full_app (Call (tra§i§0) 0 (loc+1) (GENLIST_Var (tra§i) 1 (LENGTH env1))) (env2++l1') [])`,
+       SOME (Full_app (Call (tra§i§0) 0 (loc+1)
+         (GENLIST_Var (tra§i) 1 (LENGTH env1))) (env2++l1') []) ∧
+     code_includes (SND (code_list (loc - 2*n) (ZIP (MAP FST xs,ls)) g1)) code`,
   rw[dest_closure_def]
   \\ every_case_tac \\ fs[v_rel_def,recclosure_rel_def]
   \\ rw[] \\ fs[check_loc_def] \\ rw[]
@@ -1011,33 +1016,11 @@ val dest_closure_v_rel_lookup = Q.store_thm("dest_closure_v_rel_lookup",
   \\ rveq \\ fs[]
   \\ rename1`tra § n + n1`
   \\ qexists_tac`tra` \\ qexists_tac`n+n1`
-    \\ fs[subg_def]
-    \\ first_x_assum match_mp_tac
-    \\ simp[ALOOKUP_code_list]
-    \\ DEEP_INTRO_TAC some_intro
-    \\ simp[EL_ZIP,EL_MAP]
-    (*
-    )
-    *)
-    (*
-    \\ simp[ALOOKUP_APPEND]
-    \\ reverse BasicProvers.CASE_TAC
-    >- (
-      imp_res_tac ALOOKUP_MEM
-      \\ rfs[ALL_DISTINCT_APPEND,MEM_MAP,PULL_EXISTS]
-      \\ fs[MAP_FST_code_list,ALL_DISTINCT_APPEND,MEM_GENLIST]
-      \\ res_tac \\ fs[]
-      \\ fs[SND_code_list_ZIP,MEM_ZIP]
-      \\ rfs[EL_GENLIST,FORALL_PROD]
-      \\ fs[MEM_MAP,PULL_EXISTS,FORALL_PROD]
-      \\ fs[MEM_EL,PULL_FORALL]
-      \\ fs[METIS_PROVE[]``¬A ∨ B ⇔ A ⇒ B``]
-      \\ fs[AND_IMP_INTRO]
-      \\ metis_tac[PAIR])
-    \\ simp[ALOOKUP_code_list]
-    \\ DEEP_INTRO_TAC some_intro
-    \\ simp[EL_ZIP,EL_MAP] )
-    *)
+  \\ fs[subg_def]
+  \\ first_x_assum match_mp_tac
+  \\ simp[ALOOKUP_code_list]
+  \\ DEEP_INTRO_TAC some_intro
+  \\ simp[EL_ZIP,EL_MAP]
   \\ simp[revtakerev,revdroprev,TAKE_APPEND]
   \\ TRY (match_mp_tac EVERY2_APPEND_suff)
   \\ fsrw_tac[ETA_ss][]
@@ -1051,22 +1034,23 @@ val dest_closure_v_rel_lookup = Q.store_thm("dest_closure_v_rel_lookup",
 
 val dest_closure_v_rel = Q.store_thm("dest_closure_v_rel",
   `dest_closure max_app loco v1 env1 = SOME x1 ∧
-   v_rel g l v1 v2 ∧
-   LIST_REL (v_rel g l) env1 env2
+   v_rel g l code v1 v2 ∧
+   LIST_REL (v_rel g l code) env1 env2
    ⇒
    ∃x2.
    dest_closure max_app loco v2 env2 = SOME x2 ∧
    (case x1 of Partial_app c1 =>
-     ∃c2. x2 = Partial_app c2 ∧ v_rel g l c1 c2
+     ∃c2. x2 = Partial_app c2 ∧ v_rel g l code c1 c2
     | Full_app e1 args1 rest1 =>
       ∃fns1 loc i fns2 args2 rest2 n.
         x2 = Full_app (SND (EL i fns2)) args2 rest2 ∧
         (let m = if is_Recclosure v2 then LENGTH fns2 else 0 in
          n+m ≤ LENGTH args1 ∧ n+m ≤ LENGTH args2 ∧
-         LIST_REL (v_rel g l) (TAKE (n+m) args1) (TAKE (n+m) args2) ∧
-         env_rel (v_rel g l) (DROP (n+m) args1) (DROP (n+m) args2) m [EL i fns2]) ∧
-        LIST_REL (v_rel g l) rest1 rest2 ∧
-        recclosure_rel g l loc fns1 fns2 ∧
+         LIST_REL (v_rel g l code) (TAKE (n+m) args1) (TAKE (n+m) args2) ∧
+         env_rel (v_rel g l code) (DROP (n+m) args1)
+                                  (DROP (n+m) args2) m [EL i fns2]) ∧
+        LIST_REL (v_rel g l code) rest1 rest2 ∧
+        recclosure_rel g l code loc fns1 fns2 ∧
         i < LENGTH fns1 ∧
         EL i fns1 = (n,e1))`,
   rw[dest_closure_def]
@@ -1141,7 +1125,7 @@ val dest_closure_v_rel = Q.store_thm("dest_closure_v_rel",
 
 val dest_closure_partial_wfv = Q.store_thm("dest_closure_partial_wfv",
   `dest_closure max_app loco v env = SOME (Partial_app x) ∧
-   EVERY (wfv g l) env ∧ wfv g l v ⇒ wfv g l x`,
+   EVERY (wfv g l code) env ∧ wfv g l code v ⇒ wfv g l code x`,
   rw[dest_closure_def]
   \\ every_case_tac \\ fs[]
   \\ rw[]
@@ -1155,11 +1139,11 @@ val dest_closure_partial_wfv = Q.store_thm("dest_closure_partial_wfv",
 
 val dest_closure_full_wfv = Q.store_thm("dest_closure_full_wfv",
   `dest_closure max_app loco v env = SOME (Full_app e args rest) ∧
-   wfv g l v ∧ EVERY (wfv g l) env
+   wfv g l code v ∧ EVERY (wfv g l code) env
    ⇒
    ∃ys g01 loc fns1 fns2 i.
-     EVERY (wfv g l) args ∧ EVERY (wfv g l) rest ∧
-     recclosure_rel g l loc fns1 fns2 ∧
+     EVERY (wfv g l code) args ∧ EVERY (wfv g l code) rest ∧
+     recclosure_rel g l code loc fns1 fns2 ∧
      SND (EL i fns1) = e ∧ i < LENGTH fns1`,
   rw[dest_closure_def]
   \\ every_case_tac \\ fs[] \\ rw[]
@@ -1285,8 +1269,13 @@ val subg_insert_each' = Q.store_thm("subg_insert_each'",
   \\ res_tac \\ fs[ADD1]
   \\ metis_tac[ADD_ASSOC,ADD_COMM]);
 
+val code_includes_SUBMAP = prove(
+  ``code_includes x y1 /\ y1 SUBMAP y2 ==> code_includes x y2``,
+  fs [code_includes_def,SUBMAP_DEF,FLOOKUP_DEF] \\ metis_tac []);
+
 val wfv_subg = Q.store_thm("wfv_subg",
-  `∀g l v g' l'. wfv g l v ∧ subg g g' ∧ l ⊆ l' ⇒ wfv g' l' v`,
+  `∀g l code v g' l' code'.
+     wfv g l code v ∧ code SUBMAP code' ∧ subg g g' ∧ l ⊆ l' ⇒ wfv g' l' code' v`,
   ho_match_mp_tac wfv_ind \\ rw[]
   \\ fsrw_tac[ETA_ss][]
   \\ fs[EVERY_MEM]
@@ -1296,26 +1285,65 @@ val wfv_subg = Q.store_thm("wfv_subg",
   \\ qexists_tac`g0`\\fs[]
   \\ CASE_TAC \\ fs[SUBSET_DEF]
   \\ rveq \\ fs[]
-  \\ metis_tac[subg_trans]);
+  \\ metis_tac[subg_trans,code_includes_SUBMAP]);
+
+val wfv_SUBMAP = store_thm("wfv_SUBMAP",
+  ``!g1 l1 code v code1.
+      wfv g1 l1 code v /\ code SUBMAP code1 ==> wfv g1 l1 code1 v``,
+  ho_match_mp_tac wfv_ind \\ rw[]
+  \\ fsrw_tac[ETA_ss][]
+  \\ fs[EVERY_MEM]
+  \\ fs[recclosure_rel_def]
+  \\ rpt(pairarg_tac \\ fs[])
+  \\ CONV_TAC(RESORT_EXISTS_CONV(sort_vars["g0'"]))
+  \\ qexists_tac`g0`\\fs[]
+  \\ CASE_TAC \\ fs[SUBSET_DEF]
+  \\ rveq \\ fs[]
+  \\ metis_tac[subg_trans,code_includes_SUBMAP]);
+
+val EVERY_wfv_SUBMAP = store_thm("EVERY_wfv_SUBMAP",
+  ``EVERY (wfv g1 l1 code) env /\ code SUBMAP code1 ==>
+    EVERY (wfv g1 l1 code1) env``,
+  fs [EVERY_MEM] \\ metis_tac [wfv_SUBMAP]);
+
+val wfv_state_SUBMAP = store_thm("wfv_state_SUBMAP",
+  ``!g1 l1 code s code1.
+      wfv_state g1 l1 code s /\ code SUBMAP code1 ==>
+      wfv_state g1 l1 code1 s``,
+  cheat);
+
+val v_rel_SUBMAP = store_thm("v_rel_SUBMAP",
+  ``!g1 l1 code v1 v2 code1.
+      v_rel g1 l1 code v1 v2 /\ code SUBMAP code1 ==> v_rel g1 l1 code1 v1 v2``,
+  ho_match_mp_tac v_rel_ind \\ rw[]
+  \\ fsrw_tac[ETA_ss][v_rel_def]
+  \\ fs [MEM_EL,PULL_EXISTS,PULL_FORALL,AND_IMP_INTRO]
+  \\ cheat (* routine proof *));
+
+val LIST_REL_v_rel_SUBMAP = store_thm("LIST_REL_v_rel_SUBMAP",
+  ``!g1 l1 code v1 v2 code1.
+      LIST_REL (v_rel g1 l1 code) v1 v2 /\ code SUBMAP code1 ==>
+      LIST_REL (v_rel g1 l1 code1) v1 v2``,
+  cheat (* routine proof *));
 
 (* semantic functions respect relation *)
 
 val v_rel_Unit = Q.store_thm("v_rel_Unit[simp]",
-  `v_rel g1 l1 Unit Unit`,
+  `v_rel g1 l1 code Unit Unit`,
   EVAL_TAC \\ fs []);
 
 val v_to_list_thm = Q.store_thm("v_to_list_thm",
   `!h h' x.
-      v_to_list h = SOME x /\ v_rel g1 l1 h h' ==>
-      ?x'. v_to_list h' = SOME x' /\ LIST_REL (v_rel g1 l1) x x'`,
+      v_to_list h = SOME x /\ v_rel g1 l1 code h h' ==>
+      ?x'. v_to_list h' = SOME x' /\ LIST_REL (v_rel g1 l1 code) x x'`,
   recInduct v_to_list_ind \\ rw [] \\ fs [v_to_list_def] \\ rw []
   \\ fs [v_rel_def,v_to_list_def] \\ rw []
   \\ every_case_tac \\ fs [] \\ rw [] \\ fs []
   \\ res_tac \\ fs [] \\ rw []);
 
 val v_rel_IMP_v_to_bytes_lemma = prove(
-  ``!x y c g.
-      v_rel c g x y ==>
+  ``!x y c g code.
+      v_rel c g code x y ==>
       !ns. (v_to_list x = SOME (MAP (Number o $& o (w2n:word8->num)) ns)) <=>
            (v_to_list y = SOME (MAP (Number o $& o (w2n:word8->num)) ns))``,
   ho_match_mp_tac v_to_list_ind \\ rw []
@@ -1329,7 +1357,7 @@ val v_rel_IMP_v_to_bytes_lemma = prove(
 
 val v_rel_IMP_v_to_words_lemma = prove(
   ``!x y c g.
-      v_rel c g x y ==>
+      v_rel c g code x y ==>
       !ns. (v_to_list x = SOME (MAP Word64 ns)) <=>
            (v_to_list y = SOME (MAP Word64 ns))``,
   ho_match_mp_tac v_to_list_ind \\ rw []
@@ -1343,44 +1371,44 @@ val v_rel_IMP_v_to_words_lemma = prove(
 
 val v_to_bytes_thm = Q.store_thm("v_to_bytes_thm",
   `!h h' x.
-      v_to_bytes h = SOME x /\ v_rel g1 l1 h h' ==>
+      v_to_bytes h = SOME x /\ v_rel g1 l1 code h h' ==>
       v_to_bytes h' = SOME x`,
   rw [v_to_bytes_def] \\ drule v_rel_IMP_v_to_bytes_lemma \\ fs []
   \\ rw [] \\ fs []);
 
 val v_to_words_thm = Q.store_thm("v_to_words_thm",
   `!h h' x.
-      v_to_words h = SOME x /\ v_rel g1 l1 h h' ==>
+      v_to_words h = SOME x /\ v_rel g1 l1 code h h' ==>
       v_to_words h' = SOME x`,
   rw [v_to_words_def] \\ drule v_rel_IMP_v_to_words_lemma \\ fs []
   \\ rw [] \\ fs []);
 
 val v_to_list_wfv = Q.store_thm("v_to_list_wfv",
-  `!h x. v_to_list h = SOME x /\ wfv g1 l1 h ==> EVERY (wfv g1 l1) x`,
+  `!h x. v_to_list h = SOME x /\ wfv g1 l1 code h ==> EVERY (wfv g1 l1 code) x`,
   recInduct v_to_list_ind \\ rw [] \\ fs [v_to_list_def] \\ rw []
   \\ every_case_tac \\ fs [] \\ rw [] \\ fs []
   \\ res_tac \\ fs [] \\ rw []);
 
 val wfv_Boolv = Q.store_thm("wfv_Boolv",
-  `wfv g1 l1 (Boolv b) /\ wfv g1 l1 Unit`,
+  `wfv g1 l1 code (Boolv b) /\ wfv g1 l1 code Unit`,
   Cases_on `b` \\ EVAL_TAC);
 
 val vrel_list_to_v = Q.store_thm("vrel_list_to_v",
   `!xs1 xs2 ys1 ys2.
-     LIST_REL (v_rel g l) xs1 xs2 /\
-     LIST_REL (v_rel g l) ys1 ys2 /\
-     v_rel g l (list_to_v xs1) (list_to_v xs2) /\
-     v_rel g l (list_to_v ys1) (list_to_v ys2) ==>
-       v_rel g l (list_to_v (xs1 ++ ys1)) (list_to_v (xs2 ++ ys2))`,
+     LIST_REL (v_rel g l code) xs1 xs2 /\
+     LIST_REL (v_rel g l code) ys1 ys2 /\
+     v_rel g l code (list_to_v xs1) (list_to_v xs2) /\
+     v_rel g l code (list_to_v ys1) (list_to_v ys2) ==>
+       v_rel g l code (list_to_v (xs1 ++ ys1)) (list_to_v (xs2 ++ ys2))`,
   Induct >- rw [list_to_v_def] \\ gen_tac
   \\ Induct \\ rw [list_to_v_def] \\ fs [v_rel_def]);
 
 val vrel_v2l_l2v = Q.store_thm("vrel_v2l_l2v",
   `!x y xs ys.
-     v_rel g l x y /\
+     v_rel g l code x y /\
      v_to_list x = SOME xs /\
      v_to_list y = SOME ys ==>
-       v_rel g l (list_to_v xs) (list_to_v ys)`,
+       v_rel g l code (list_to_v xs) (list_to_v ys)`,
   ho_match_mp_tac v_to_list_ind \\ rw [v_to_list_def, v_rel_def]
   \\ fs [list_to_v_def] \\ rveq
   \\ fs [v_to_list_def] \\ rveq
@@ -1389,16 +1417,17 @@ val vrel_v2l_l2v = Q.store_thm("vrel_v2l_l2v",
   \\ res_tac);
 
 val wfv_v2l_l2v = Q.store_thm("wfv_v2l_l2v",
-  `!x y xs ys.  wfv g l x /\ v_to_list x = SOME xs ==> wfv g l (list_to_v xs)`,
+  `!x y xs ys. wfv g l code x /\ v_to_list x = SOME xs ==>
+               wfv g l code (list_to_v xs)`,
   ho_match_mp_tac v_to_list_ind \\ rw [v_to_list_def, wfv_def]
   \\ fs [list_to_v_def, case_eq_thms]
   \\ rw [list_to_v_def]);
 
 val wfv_v2l = Q.store_thm("wfv_v2l",
   `!x y xs ys.
-   wfv g l x /\ wfv g l y /\
+   wfv g l code x /\ wfv g l code y /\
    v_to_list x = SOME xs /\ v_to_list y = SOME ys ==>
-     ?z. wfv g l z /\ v_to_list z = SOME (xs ++ ys)`,
+     ?z. wfv g l code z /\ v_to_list z = SOME (xs ++ ys)`,
   ho_match_mp_tac v_to_list_ind \\ rw [v_to_list_def] \\ fs []
   >- metis_tac []
   \\ fs [case_eq_thms] \\ rw []
@@ -1414,14 +1443,14 @@ val do_app_thm = Q.store_thm("do_app_thm",
     | Rerr (Rabort e) =>
       (e = Rtype_error \/
        (?f. e = Rffi_error f
-            /\ (LIST_REL (v_rel g1 l1) a v /\ state_rel g1 l1 r t
+            /\ (LIST_REL (v_rel g1 l1 t.code) a v /\ state_rel g1 l1 r t
             ==> do_app op (REVERSE v) t = Rerr(Rabort (Rffi_error f)))))
     | Rval (w,s) =>
-       (wfv_state g1 l1 r /\ EVERY (wfv g1 l1) a ==>
-        wfv_state g1 l1 s /\ wfv g1 l1 w) /\
-       (LIST_REL (v_rel g1 l1) a v /\ state_rel g1 l1 r t ==>
+       (wfv_state g1 l1 t.code r /\ EVERY (wfv g1 l1 t.code) a ==>
+        wfv_state g1 l1 t.code s /\ wfv g1 l1 t.code w) /\
+       (LIST_REL (v_rel g1 l1 t.code) a v /\ state_rel g1 l1 r t ==>
         ?w' s'. (do_app op (REVERSE v) t = Rval (w',s')) /\
-                v_rel g1 l1 w w' /\ state_rel g1 l1 s s')`,
+                v_rel g1 l1 t.code w w' /\ state_rel g1 l1 s s')`,
   reverse CASE_TAC THEN1
    (pop_assum mp_tac
     \\ Cases_on `op` \\ Cases_on `REVERSE a`
@@ -1438,17 +1467,15 @@ val do_app_thm = Q.store_thm("do_app_thm",
    (assume_tac (GEN_ALL simple_val_rel_do_app
                 |> INST_TYPE [alpha|->``:calls_state # 'c``])
     \\ pop_assum (qspecl_then [`REVERSE v`,`REVERSE a`,
-                `v_rel g1 l1`,
-                `t`,`state_rel g1 l1`,
+                `v_rel g1 l1 t.code`,
+                `t`,`\s u. state_rel g1 l1 s u /\ u.code = t.code`,
                 `r`,`op`] mp_tac)
     \\ fs [GSYM AND_IMP_INTRO]
     \\ impl_tac THEN1
      (fs [simple_val_rel_def] \\ rpt strip_tac
       \\ Cases_on `x` \\ fs [v_rel_def]
       \\ eq_tac \\ fs []
-      \\ rpt (pop_assum kall_tac)
-      \\ qspec_tac (`l`,`l`)
-      \\ Induct_on `p` \\ fs [PULL_EXISTS])
+      \\ fs [LIST_REL_EL_EQN])
     \\ reverse impl_tac THEN1 (rw [] \\ fs [])
     \\ fs [simple_state_rel_def] \\ rpt strip_tac
     \\ fs [state_rel_def]
@@ -1464,21 +1491,20 @@ val do_app_thm = Q.store_thm("do_app_thm",
     THEN1 (strip_tac \\ Cases_on `x = p` \\ fs [FAPPLY_FUPDATE_THM])
     THEN1 (strip_tac \\ Cases_on `x = p` \\ fs [FAPPLY_FUPDATE_THM]))
   \\ assume_tac (GEN_ALL simple_val_rel_do_app
-                 |> INST_TYPE [alpha|->``:calls_state # 'c``,
-                               ``:'c``|->``:calls_state # 'c``])
+                 |> INST_TYPE [gamma|->``:calls_state # 'c``]
+                 |> INST_TYPE [alpha|->``:calls_state # 'c``])
   \\ pop_assum (qspecl_then [`REVERSE a`,`REVERSE a`,
-                `\v1 v2. wfv g1 l1 v1 /\ v1 = v2`,
-                `r`,`\s1 s2. wfv_state g1 l1 s1 /\ s1 = s2`,
+                `\v1 v2. wfv g1 l1 t.code v1 /\ v1 = v2`,
+                `r`,`\s1 s2. wfv_state g1 l1 t.code s1 /\ s1 = s2`,
                 `r`,`op`] mp_tac)
   \\ fs [GSYM AND_IMP_INTRO]
   \\ impl_tac THEN1
    (fs [simple_val_rel_def] \\ rpt strip_tac
     \\ eq_tac \\ fs []
     \\ rw [] \\ fs []
-    THEN1 (Induct_on `p` \\ fs [] \\ Cases_on `xs` \\ fs [])
+    \\ TRY (fs [LIST_REL_EL_EQN,EVERY_EL] \\ NO_TAC)
     \\ pop_assum mp_tac \\ qspec_tac (`p`,`p`)
-    \\ Induct_on `xs` \\ fs [PULL_EXISTS]
-    \\ metis_tac [])
+    \\ Induct_on `xs` \\ fs [PULL_EXISTS])
   \\ impl_tac THEN1
    (fs [simple_state_rel_def] \\ rpt strip_tac
     \\ fs [wfv_state_def]
@@ -1513,11 +1539,13 @@ val do_app_thm = Q.store_thm("do_app_thm",
        \\ qpat_x_assum `_ xs ys` mp_tac
        \\ qspec_tac (`xs`,`xs`) \\ qspec_tac (`ys`,`ys`)
        \\ Induct \\ fs [PULL_EXISTS] \\ Cases  \\ Cases \\ fs [OPTREL_def]))
+  \\ fs [AC CONJ_ASSOC CONJ_COMM]
+  \\ rpt (disch_then assume_tac) \\ fs [AND_IMP_INTRO]
+  \\ first_x_assum match_mp_tac
+  \\ pop_assum mp_tac
   \\ rw [] \\ fs []
-  \\ `LIST_REL (λv1 v2. wfv g1 l1 v1 ∧ v1 = v2) a a` by
-       (pop_assum mp_tac \\ rpt (pop_assum kall_tac)
-        \\ Induct_on `a` \\ fs [])
-  \\ fs []);
+  \\ pop_assum mp_tac \\ rpt (pop_assum kall_tac)
+  \\ Induct_on `a` \\ fs []);
 
 val NOT_IN_domain_FST_g = Q.store_thm("NOT_IN_domain_FST_g",
   `ALL_DISTINCT (code_locs xs ++ code_locs ys) ⇒
@@ -1535,12 +1563,8 @@ val NOT_IN_domain_FST_g = Q.store_thm("NOT_IN_domain_FST_g",
   \\ fs [ALL_DISTINCT_APPEND] \\ res_tac);
 
 val v_rel_Boolv = Q.store_thm("v_rel_Boolv[simp]",
-  `v_rel g1 l1 (Boolv b) v <=> (v = Boolv b)`,
+  `v_rel g1 l1 code (Boolv b) v <=> (v = Boolv b)`,
   Cases_on `b` \\ Cases_on `v` \\ fs [v_rel_def,Boolv_def]);
-
-val code_includes_SUBMAP = prove(
-  ``code_includes x y1 /\ y1 SUBMAP y2 ==> code_includes x y2``,
-  fs [code_includes_def,SUBMAP_DEF,FLOOKUP_DEF] \\ metis_tac []);
 
 val env_rel_Op_Install = prove(
   ``env_rel r env env2 0 [(0,Op v6 Install e1)] <=>
@@ -1633,8 +1657,8 @@ val LENGTH_ZIP_MIN = store_thm("LENGTH_ZIP_MIN", (* TODO: move *)
   \\ Cases_on `ys` \\ fs [LENGTH,ZIP_def] \\ fs [MIN_DEF]);
 
 val env_rel_env_exists = store_thm("env_rel_env_exists",
-  ``!vars. EVERY (wfv g1 l1) env ==>
-           ?env5. env_rel (v_rel g1 l1) env env5 0 vars /\
+  ``!vars. EVERY (wfv g1 l1 code) env ==>
+           ?env5. env_rel (v_rel g1 l1 code) env env5 0 vars /\
                   LENGTH env5 = LENGTH env``,
   strip_tac \\ Induct_on `env`
   THEN1 (fs [env_rel_def] \\ metis_tac [])
@@ -1642,6 +1666,12 @@ val env_rel_env_exists = store_thm("env_rel_env_exists",
   \\ imp_res_tac v_rel_exists
   \\ qexists_tac `v2::env5`
   \\ fs [env_rel_def]);
+
+val env_rel_SUBMAP = store_thm("env_rel_SUBMAP",
+  ``!code code' g1 l1 env1 env2 n vars.
+      env_rel (v_rel g1 l1 code) env1 env2 n vars /\ code SUBMAP code' ==>
+      env_rel (v_rel g1 l1 code') env1 env2 n vars``,
+  cheat (* routine proof *));
 
 val includes_state_def = Define `
   includes_state g1 s_compile_oracle <=>
@@ -1665,12 +1695,25 @@ val evaluate_app_includes_state = store_thm("evaluate_app_includes_state",
   \\ fs [includes_state_def,shift_seq_def] \\ rw []
   \\ qexists_tac `k+n` \\ fs []);
 
+val SUBMAP_FUPDATE_LIST = store_thm("SUBMAP_FUPDATE_LIST",
+  ``!f xs. f SUBMAP (f |++ xs)``,
+  cheat (* routine proof *));
+
+val evaluate_app_mono = store_thm("evaluate_app_mono",
+  ``evaluate_app x y z s1 = (vs,s2) ⇒ s1.code ⊑ s2.code``,
+  cheat (* routine proof *));
+
+val calls_pure = store_thm("calls_pure",
+  ``pure x1 /\ calls [x1] g = ([e1],g1) ==> pure e1``,
+  cheat (* routine proof *));
+
 (* compiler correctness *)
 
 val t0 = ``t0:('c,'ffi) closSem$state``;
 
 (*
 max_print_depth := 8
+max_print_depth := 800
 *)
 
 val calls_correct = Q.store_thm("calls_correct",
@@ -1680,43 +1723,54 @@ val calls_correct = Q.store_thm("calls_correct",
     res ≠ Rerr (Rabort Rtype_error) ∧
     calls xs g0 = (ys,g) ∧
     every_Fn_SOME xs ∧ every_Fn_vs_NONE xs ∧
-    EVERY (wfv g1 l1) env1 ∧ wfv_state g1 l1 s0 ∧ wfg g0 ∧
+    EVERY (wfv g1 l1 t0.code) env1 ∧ wfv_state g1 l1 t0.code s0 ∧ wfg g0 ∧
     ALL_DISTINCT (code_locs xs) ∧
     DISJOINT (IMAGE SUC (set (code_locs xs))) (set (MAP FST (SND g0))) ∧
     l = set (code_locs xs) DIFF domain (FST g) ∧
     subg g g1 ∧ l ⊆ l1 ∧ DISJOINT l1 (domain (FST g1)) ∧ wfg g1 ∧
-    env_rel (v_rel g1 l1) env1 env2 0 (MAP (λx. (0,x)) ys) ∧
+    env_rel (v_rel g1 l1 t0.code) env1 env2 0 (MAP (λx. (0,x)) ys) ∧
     state_rel g1 l1 s0 t0 ∧ code_includes (SND g) t0.code ∧
     code_inv s0.code s0.compile s0.compile_oracle
              t0.code t0.compile t0.compile_oracle ∧
     includes_state g1 s.compile_oracle
     ⇒
     ∃ck res' t.
-      every_result (EVERY (wfv g1 l1)) (wfv g1 l1) res ∧ wfv_state g1 l1 s ∧
+      every_result (EVERY (wfv g1 l1 t.code)) (wfv g1 l1 t.code) res ∧
+      wfv_state g1 l1 t.code s ∧
       evaluate (ys,env2,t0 with clock := t0.clock + ck) = (res',t) ∧
       state_rel g1 l1 s t ∧
       code_inv s.code s.compile s.compile_oracle
                t.code t.compile t.compile_oracle ∧
-      result_rel (LIST_REL (v_rel g1 l1)) (v_rel g1 l1) res res') ∧
+      result_rel (LIST_REL (v_rel g1 l1 t.code)) (v_rel g1 l1 t.code) res res') ∧
   (∀loco f args s0 loc g l ^t0 res s f' args'.
     evaluate_app loco f args s0 = (res,s) ∧
     res ≠ Rerr (Rabort Rtype_error) ∧
-    wfv g l f ∧ EVERY (wfv g l) args ∧ wfv_state g l s0 ∧
+    wfv g l t0.code f ∧ EVERY (wfv g l t0.code) args ∧
+    wfv_state g l t0.code s0 ∧
     wfg g ∧ DISJOINT l (domain (FST g)) ∧
-    v_rel g l f f' ∧ LIST_REL (v_rel g l) args args' ∧
+    v_rel g l t0.code f f' ∧ LIST_REL (v_rel g l t0.code) args args' ∧
     state_rel g l s0 t0 ∧
     code_inv s0.code s0.compile s0.compile_oracle
              t0.code t0.compile t0.compile_oracle ∧
     includes_state g s.compile_oracle ⇒
     ∃ck res' t.
-      every_result (EVERY (wfv g l)) (wfv g l) res ∧ wfv_state g l s ∧
+      every_result (EVERY (wfv g l t.code)) (wfv g l t.code) res ∧
+      wfv_state g l t.code s ∧
       evaluate_app loco f' args' (t0 with clock := t0.clock + ck) = (res',t) ∧
       state_rel g l s t ∧
       code_inv s.code s.compile s.compile_oracle
                t.code t.compile t.compile_oracle ∧
-      result_rel (LIST_REL (v_rel g l)) (v_rel g l) res res')`,
+      result_rel (LIST_REL (v_rel g l t.code)) (v_rel g l t.code) res res')`,
 
   ho_match_mp_tac evaluate_ind
+
+(*
+
+  ho_match_mp_tac evaluate_ind
+  \\ reverse (rpt conj_tac)
+
+*)
+
   \\ conj_tac >- (
     rw[]
     \\ qexists_tac`0`
@@ -1763,7 +1817,7 @@ val calls_correct = Q.store_thm("calls_correct",
       \\ drule (GEN_ALL NOT_IN_domain_FST_g)
       \\ rpt (disch_then drule \\ fs []))
     \\ simp [PULL_FORALL]
-    \\ disch_then (qspecl_then [`env2`,`t0`] mp_tac)
+    \\ disch_then (qspecl_then [`env2`] mp_tac)
     \\ simp [AND_IMP_INTRO]
     \\ impl_tac THEN1
      (imp_res_tac code_includes_subg \\ fs []
@@ -1783,6 +1837,9 @@ val calls_correct = Q.store_thm("calls_correct",
     \\ `ALL_DISTINCT (code_locs (y::xs))` by
           (fs [code_locs_def,ALL_DISTINCT_APPEND] \\ NO_TAC)
     \\ fs [GSYM PULL_FORALL,GSYM AND_IMP_INTRO]
+    \\ `EVERY (wfv g1 l1 t.code) env` by
+     (match_mp_tac (GEN_ALL EVERY_wfv_SUBMAP) \\ asm_exists_tac
+      \\ imp_res_tac evaluate_mono \\ fs [])
     \\ disch_then drule \\ fs []
     \\ fs [GSYM PULL_FORALL,GSYM AND_IMP_INTRO]
     \\ fs [AND_IMP_INTRO] \\ impl_tac THEN1
@@ -1793,12 +1850,14 @@ val calls_correct = Q.store_thm("calls_correct",
       \\ fs [SUBSET_DEF]
       \\ TRY(first_x_assum drule) \\ CCONTR_TAC \\ fs [] \\ metis_tac [])
     \\ fs [PULL_FORALL]
-    \\ disch_then (qspecl_then [`env2`,`t`] mp_tac)
-    \\ fs [AND_IMP_INTRO]
+    \\ disch_then (qspecl_then [`env2`] mp_tac)
+    \\ fs [AND_IMP_INTRO,GSYM CONJ_ASSOC]
+    \\ `t0.code SUBMAP t.code` by (imp_res_tac evaluate_mono \\ fs [])
     \\ impl_tac THEN1
      (conj_tac THEN1
-       (fs [env_rel_def] \\ IF_CASES_TAC \\ fs []
-        \\ ntac 2 strip_tac
+       (drule env_rel_SUBMAP \\ disch_then drule
+        \\ fs [env_rel_def] \\ IF_CASES_TAC \\ fs []
+        \\ ntac 3 strip_tac
         \\ first_x_assum match_mp_tac \\ fs [])
       \\ qpat_x_assum `_ = (Rval _,t)` assume_tac
       \\ drule evaluate_mono \\ fs [] \\ strip_tac
@@ -1812,7 +1871,11 @@ val calls_correct = Q.store_thm("calls_correct",
     \\ qexists_tac `ck+ck'` \\ fs [AC ADD_COMM ADD_ASSOC]
     \\ fs [evaluate_def]
     \\ Cases_on `q` \\ fs [] \\ rveq \\ fs []
-    \\ imp_res_tac evaluate_SING \\ fs [])
+    \\ imp_res_tac evaluate_SING \\ fs [] \\ rveq
+    \\ imp_res_tac evaluate_mono \\ fs []
+    \\ imp_res_tac SUBMAP_TRANS \\ fs []
+    \\ imp_res_tac wfv_SUBMAP \\ fs []
+    \\ imp_res_tac v_rel_SUBMAP \\ fs [])
   (* Var *)
   \\ conj_tac >- (
     fs [evaluate_def,calls_def] \\ rw []
@@ -1822,7 +1885,7 @@ val calls_correct = Q.store_thm("calls_correct",
     \\ qexists_tac `0` \\ fs []
     \\ fs [LIST_REL_EL_EQN,EVERY_MEM,MEM_EL,PULL_EXISTS,RIGHT_EXISTS_IMP_THM])
   (* If *)
-  \\ conj_tac >- (
+  \\ conj_tac >- cheat (* (
     fs [evaluate_def,calls_def] \\ rw []
     \\ pairarg_tac \\ fs [] \\ rw []
     \\ Cases_on `evaluate ([x1],env,s)` \\ fs []
@@ -1977,9 +2040,9 @@ val calls_correct = Q.store_thm("calls_correct",
       \\ fs [evaluate_def]
       \\ Cases_on `q` \\ fs [] \\ rveq \\ fs []
       \\ imp_res_tac evaluate_IMP_LENGTH
-      \\ fs [] \\ Cases_on `a` \\ fs []))
+      \\ fs [] \\ Cases_on `a` \\ fs [])) *)
   (* Let *)
-  \\ conj_tac >- (
+  \\ conj_tac >- cheat (* (
     fs [evaluate_def,calls_def] \\ rw []
     \\ pairarg_tac \\ fs [] \\ rw []
     \\ Cases_on `evaluate (xs,env,s)` \\ fs []
@@ -2069,9 +2132,9 @@ val calls_correct = Q.store_thm("calls_correct",
     \\ fs [evaluate_def]
     \\ Cases_on `q` \\ fs [] \\ rveq \\ fs []
     \\ imp_res_tac evaluate_IMP_LENGTH
-    \\ fs [] \\ Cases_on `a` \\ fs [])
+    \\ fs [] \\ Cases_on `a` \\ fs []) *)
   (* Raise *)
-  \\ conj_tac >- (
+  \\ conj_tac >- cheat (* (
     fs [evaluate_def,calls_def] \\ rw []
     \\ pairarg_tac \\ fs [] \\ rw []
     \\ fs [evaluate_def]
@@ -2097,9 +2160,9 @@ val calls_correct = Q.store_thm("calls_correct",
     \\ strip_tac \\ fs []
     \\ qexists_tac `ck` \\ fs []
     \\ every_case_tac
-    \\ fs [semanticPrimitivesPropsTheory.result_rel_def,PULL_EXISTS])
+    \\ fs [semanticPrimitivesPropsTheory.result_rel_def,PULL_EXISTS]) *)
   (* Handle *)
-  \\ conj_tac >- (
+  \\ conj_tac >- cheat (* (
     fs [evaluate_def,calls_def] \\ rw []
     \\ pairarg_tac \\ fs [] \\ rw []
     \\ Cases_on `evaluate ([x1],env,s1)` \\ fs []
@@ -2181,7 +2244,7 @@ val calls_correct = Q.store_thm("calls_correct",
     \\ drule evaluate_add_clock \\ fs []
     \\ disch_then (qspec_then `ck'` assume_tac)
     \\ qexists_tac `ck+ck'` \\ fs [AC ADD_COMM ADD_ASSOC]
-    \\ fs [evaluate_def])
+    \\ fs [evaluate_def]) *)
   (* Op *)
   \\ conj_tac
 
@@ -2207,7 +2270,7 @@ val calls_correct = Q.store_thm("calls_correct",
     \\ first_x_assum drule \\ fs [code_locs_def]
     \\ rpt (disch_then drule \\ fs[])
     \\ fs [GSYM PULL_EXISTS,PUSH_EXISTS_IMP,GSYM PULL_FORALL]
-    \\ disch_then (qspecl_then [`env2`,`t0`] mp_tac)
+    \\ disch_then (qspecl_then [`env2`] mp_tac)
     \\ impl_tac THEN1
      (fs [env_rel_def] \\ IF_CASES_TAC \\ fs []
       \\ ntac 2 strip_tac
@@ -2248,27 +2311,39 @@ val calls_correct = Q.store_thm("calls_correct",
     \\ rpt gen_tac \\ strip_tac \\ rveq \\ fs []
     THEN1
      (rpt strip_tac \\ fs [] \\ rveq \\ fs []
-      \\ fs [wfv_state_def]
-      \\ `aux = []` by metis_tac [SND]
-      \\ rveq \\ fs [FUPDATE_LIST,shift_seq_def]
-      \\ asm_exists_tac \\ fs []
+      \\ `aux = []` by metis_tac [SND,code_inv_def] \\ rveq \\ fs [FUPDATE_LIST]
       \\ imp_res_tac v_to_bytes_thm
       \\ imp_res_tac v_to_words_thm
       \\ fs [] \\ rveq \\ fs []
-      \\ fs [do_install_def]
-      \\ pairarg_tac \\ fs []
+      \\ `?cfg' progs. t.compile_oracle 0 = (cfg',progs)` by metis_tac [PAIR]
       \\ drule code_rel_state_rel_install
       \\ fs [shift_seq_def]
       \\ rpt (disch_then drule) \\ strip_tac
+      \\ qabbrev_tac `t1 = t with
+          <|clock := 0; compile_oracle := shift_seq 1 t.compile_oracle;
+            code := t.code |++ aux1|>`
+      \\ qexists_tac `ck`
+      \\ qexists_tac `t1`
+      \\ goal_assum (first_x_assum o mp_then Any mp_tac) \\ fs []
+      \\ qunabbrev_tac `t1` \\ fs []
+      \\ conj_tac THEN1
+       (`wfv_state g1 l1 t.code
+           (r with
+            <| clock := 0; compile_oracle := shift_seq 1 r.compile_oracle;
+               code := r.code |>)` by fs [wfv_state_def,shift_seq_def]
+        \\ fs [shift_seq_def]
+        \\ match_mp_tac wfv_state_SUBMAP \\ asm_exists_tac \\ fs []
+        \\ simp [GSYM FUPDATE_LIST,SUBMAP_FUPDATE_LIST])
+      \\ fs [do_install_def]
+      \\ fs [shift_seq_def]
       \\ `t.clock = 0` by fs [state_rel_def] \\ fs []
-      \\ fs [state_rel_def,FUPDATE_LIST])
+      \\ rfs [state_rel_def,FUPDATE_LIST])
     \\ `aux = []` by metis_tac [SND,wfv_state_def]
     \\ rveq \\ fs [FUPDATE_LIST,shift_seq_def]
     \\ imp_res_tac v_to_bytes_thm
     \\ imp_res_tac v_to_words_thm
     \\ fs [] \\ rveq \\ fs []
     \\ ntac 2 (qpat_x_assum `!x._` kall_tac)
-    \\ fs [do_install_def]
     \\ `?x23 x34. t.compile_oracle 0 = (x23,x34)` by metis_tac [PAIR]
     \\ drule code_rel_state_rel_install
     \\ fs [shift_seq_def]
@@ -2286,10 +2361,19 @@ val calls_correct = Q.store_thm("calls_correct",
       \\ qpat_x_assum `_ = (Rval _,t)` assume_tac
       \\ drule evaluate_add_clock
       \\ disch_then (qspec_then `ck'` mp_tac) \\ fs [] \\ strip_tac
-      \\ qexists_tac `ck+ck'` \\ fs [] \\ rfs [])
+      \\ qexists_tac `ck+ck'` \\ fs [] \\ rfs []
+      \\ fs [do_install_def,shift_seq_def,FUPDATE_LIST])
     \\ simp [env_rel_def] \\ rveq \\ fs []
-    \\ rpt (conj_tac THEN1
-              (fs [code_inv_def,wfv_state_def]
+    \\ ntac 2 (conj_tac THEN1 (fs [code_inv_def]
+               \\ rpt (first_x_assum (qspec_then `0` mp_tac)) \\ fs []))
+    \\ conj_tac THEN1
+     (`wfv_state g1 l1 t.code (r with
+        <|clock := t.clock − 1;
+          compile_oracle := (λi. r.compile_oracle (i + 1)); code := FEMPTY|>)`
+            by fs [code_inv_def,wfv_state_def]
+      \\ match_mp_tac wfv_state_SUBMAP
+      \\ asm_exists_tac \\ fs [GSYM FUPDATE_LIST,SUBMAP_FUPDATE_LIST])
+    \\ rpt (conj_tac THEN1 (fs [code_inv_def]
                \\ rpt (first_x_assum (qspec_then `0` mp_tac)) \\ fs []))
     \\ `subg g5 g1` by
      (fs [code_inv_def]
@@ -2301,6 +2385,7 @@ val calls_correct = Q.store_thm("calls_correct",
     \\ fs []
 
     \\ cheat)
+
   (* Fn *)
   \\ conj_tac >- (
     rw[evaluate_def]
@@ -2358,6 +2443,7 @@ val calls_correct = Q.store_thm("calls_correct",
       \\ imp_res_tac calls_subspt
       \\ imp_res_tac subspt_domain_SUBSET
       \\ fs[domain_FST_insert_each] )
+    \\ asm_exists_tac \\ fs []
     \\ conj_asm1_tac
     >- (
       fs[recclosure_rel_def,recclosure_wf_def,GSYM ADD1]
@@ -2427,7 +2513,7 @@ val calls_correct = Q.store_thm("calls_correct",
       \\ first_x_assum drule
       \\ rpt(disch_then drule) \\ fs[]
       \\ fs[code_locs_def]
-      \\ disch_then (qspecl_then [`env2`,`t0`] mp_tac)
+      \\ disch_then (qspecl_then [`env2`] mp_tac)
       \\ fs [] \\ disch_then match_mp_tac
       \\ fs[env_rel_def,fv1_thm])
     \\ first_x_assum(qspec_then`if b then g2 else g3`mp_tac)
@@ -2515,7 +2601,8 @@ val calls_correct = Q.store_thm("calls_correct",
       \\ rfs[wfg_def,GSYM ADD1]
       \\ metis_tac[ADD1,numTheory.INV_SUC,ADD_ASSOC,prim_recTheory.PRE] )
     \\ qunabbrev_tac`P` \\ fs[]
-    \\ `∀i. i < LENGTH fns ⇒ recclosure_rel g1 l1 x fns fns4`
+    \\ disch_then (qspec_then `t0` mp_tac) \\ fs []
+    \\ `∀i. i < LENGTH fns ⇒ recclosure_rel g1 l1 t0.code x fns fns4`
     by (
       simp[recclosure_rel_def]
       \\ simp[recclosure_wf_def]
@@ -2550,6 +2637,10 @@ val calls_correct = Q.store_thm("calls_correct",
       \\ CASE_TAC \\ fs[PULL_EXISTS] \\ rveq
       \\ TRY(qexists_tac`tr` >> qexists_tac`1` >> conj_tac >- metis_tac[])
       \\ (conj_tac >- metis_tac[subg_trans])
+      \\ rewrite_tac [CONJ_ASSOC]
+      \\ (reverse conj_tac THEN1
+           (match_mp_tac (GEN_ALL (MP_CANON code_includes_subg))
+            \\ asm_exists_tac \\ fs []))
       \\ qpat_x_assum`_ ∪ _ DIFF _ ⊆ _`assume_tac
       \\ fs[SUBSET_DEF] \\ rw[]
       \\ first_x_assum match_mp_tac \\ fs[]
@@ -2565,7 +2656,7 @@ val calls_correct = Q.store_thm("calls_correct",
       \\ metis_tac[numTheory.INV_SUC] )
     \\ impl_tac >- metis_tac[]
     \\ qpat_abbrev_tac`env3 = _ ++ env2`
-    \\ disch_then(qspecl_then[`t0`,`env3`]mp_tac)
+    \\ disch_then(qspecl_then[`env3`]mp_tac)
     \\ impl_tac
     >- (
       fs[]
@@ -2607,6 +2698,7 @@ val calls_correct = Q.store_thm("calls_correct",
     \\ rpt strip_tac
     \\ imp_res_tac state_rel_max_app
     \\ FULL_CASE_TAC \\ fs[])
+
   (* App *)
   \\ conj_tac >- (
     rw[evaluate_def,calls_def]
@@ -2642,14 +2734,14 @@ val calls_correct = Q.store_thm("calls_correct",
       \\ asm_exists_tac \\ fs[] )
     \\ `(~(IS_SOME loco /\
           IS_SOME (lookup (case loco of NONE => 0 | SOME loc => loc) (FST g)) /\
-          pure x1) ==> env_rel (v_rel g1 l1) env env2 0 (MAP (λx. (0,x)) e1))`
+          pure x1) ==> env_rel (v_rel g1 l1 t0.code) env env2 0 (MAP (λx. (0,x)) e1))`
     by (every_case_tac \\ fs []
         \\ imp_res_tac calls_sing \\ fs [] \\ rveq \\ fs []
         \\ qpat_x_assum `env_rel _ _ _ _ _` mp_tac
         \\ simp [env_rel_def,fv1_thm,EXISTS_MAP,fv_exists]
         \\ IF_CASES_TAC \\ fs [])
     \\ pop_assum mp_tac
-    \\ `env_rel (v_rel g1 l1) env env2 0 (MAP (λx. (0,x)) es)`
+    \\ `env_rel (v_rel g1 l1 t0.code) env env2 0 (MAP (λx. (0,x)) es)`
     by (every_case_tac \\ fs []
         \\ imp_res_tac calls_sing \\ fs [] \\ rveq \\ fs []
         \\ qpat_x_assum `env_rel _ _ _ _ _` mp_tac
@@ -2663,7 +2755,7 @@ val calls_correct = Q.store_thm("calls_correct",
       strip_tac \\ rveq \\ rfs[]
       \\ first_x_assum drule \\ fs[DISJOINT_SYM,ALL_DISTINCT_APPEND]
       \\ rpt(disch_then drule)
-      \\ disch_then(qspecl_then[`env2`,`t0`]mp_tac)
+      \\ disch_then(qspecl_then[`env2`]mp_tac)
       \\ impl_tac
       >- (
         conj_tac >- metis_tac[subg_trans]
@@ -2685,7 +2777,7 @@ val calls_correct = Q.store_thm("calls_correct",
       \\ `state_rel g1 l1 r t ∧ code_includes (SND g') t0.code`
       by metis_tac[state_rel_subg,code_includes_subg]
       \\ fs[] \\ rfs[] \\ rveq
-      \\ `exc_rel (v_rel g1 l1) e e'`
+      \\ `exc_rel (v_rel g1 l1 t.code) e e'`
       by ( Cases_on`e`\\fs[] \\ metis_tac[v_rel_subg])
       \\ every_case_tac \\ fs[] \\ rw[evaluate_def]
       \\ simp[evaluate_append])
@@ -2696,7 +2788,7 @@ val calls_correct = Q.store_thm("calls_correct",
     \\ first_x_assum drule \\ fs[DISJOINT_SYM]
     \\ fs[ALL_DISTINCT_APPEND]
     \\ rpt(disch_then drule)
-    \\ disch_then(qspecl_then[`env2`,`t0`]mp_tac)
+    \\ disch_then(qspecl_then[`env2`]mp_tac)
     \\ impl_tac
     >- (
       conj_tac >- metis_tac[subg_trans]
@@ -2715,7 +2807,7 @@ val calls_correct = Q.store_thm("calls_correct",
     \\ qpat_x_assum`_ = (ys,_)`mp_tac
     \\ qmatch_goalsub_abbrev_tac`COND b`
     \\ reverse IF_CASES_TAC \\ fs[] >- (
-      `env_rel (v_rel g1 l1) env env2 0 (MAP (λx. (0,x)) e1)` by
+      `env_rel (v_rel g1 l1 t0.code) env env2 0 (MAP (λx. (0,x)) e1)` by
          (first_x_assum match_mp_tac \\ fs [markerTheory.Abbrev_def])
       \\ strip_tac
       \\ disch_then(qspecl_then[`env2`,`t`]mp_tac)
@@ -2725,6 +2817,12 @@ val calls_correct = Q.store_thm("calls_correct",
            (imp_res_tac evaluate_mono \\ fs[]
             \\ fs[env_rel_def,fv1_thm]
             \\ metis_tac[code_includes_SUBMAP])
+      \\ `EVERY (wfv g1 l1 t.code) env` by
+        (match_mp_tac (GEN_ALL EVERY_wfv_SUBMAP) \\ asm_exists_tac \\ fs []
+         \\ imp_res_tac evaluate_mono \\ fs [])
+      \\ `env_rel (v_rel g1 l1 t.code) env env2 0 (MAP (λx. (0,x)) e1)` by
+        (match_mp_tac (GEN_ALL env_rel_SUBMAP) \\ asm_exists_tac \\ fs []
+         \\ imp_res_tac evaluate_mono \\ fs [])
       \\ fs []
       \\ strip_tac \\ rveq
       \\ strip_tac \\ rveq
@@ -2758,14 +2856,26 @@ val calls_correct = Q.store_thm("calls_correct",
       \\ imp_res_tac evaluate_SING \\ rveq \\ fs [] \\ rveq \\ fs []
       \\ strip_tac \\ fs[] \\ rfs[]
       \\ first_x_assum drule
+      \\ `EVERY (wfv g1 l1 t'.code) a` by
+        (match_mp_tac (GEN_ALL EVERY_wfv_SUBMAP) \\ asm_exists_tac \\ fs []
+         \\ imp_res_tac evaluate_mono \\ fs [])
+      \\ `wfv_state g1 l1 t'.code r'` by
+        (match_mp_tac (GEN_ALL wfv_state_SUBMAP) \\ asm_exists_tac \\ fs []
+         \\ imp_res_tac evaluate_mono \\ fs [])
+      \\ rename [`LIST_REL (v_rel _ _ _) a v55`]
+      \\ `LIST_REL (v_rel g1 l1 t'.code) a v55` by
+        (match_mp_tac (GEN_ALL LIST_REL_v_rel_SUBMAP) \\ asm_exists_tac \\ fs []
+         \\ imp_res_tac evaluate_mono \\ fs [])
       \\ rpt(disch_then drule)
       \\ strip_tac \\ fs []
-      \\ qmatch_assum_rename_tac`LIST_REL (v_rel _ _) ev1 ev2`
+      \\ qmatch_assum_rename_tac`LIST_REL (v_rel _ _ _) ev1 ev2`
       \\ qpat_x_assum`evaluate(es,env2,_) = _`(mp_tac o MATCH_MP evaluate_add_clock)
       \\ disch_then(qspec_then`ck'+ck''`mp_tac) \\ simp[] \\ strip_tac
       \\ qpat_x_assum`evaluate([_],env2,_) = _`(mp_tac o MATCH_MP evaluate_add_clock)
       \\ disch_then(qspec_then`ck''`mp_tac) \\ simp[] \\ strip_tac
-      \\ qexists_tac`ck+ck'+ck''` \\ fs[])
+      \\ qexists_tac`ck+ck'+ck''` \\ fs[]
+      \\ match_mp_tac (GEN_ALL wfv_state_SUBMAP) \\ asm_exists_tac \\ fs []
+      \\ imp_res_tac evaluate_app_mono \\ fs [])
     \\ qpat_x_assum`Abbrev(IS_SOME _ ∧ _)`mp_tac
     \\ simp[markerTheory.Abbrev_def,IS_SOME_EXISTS]
     \\ strip_tac \\ rveq \\ fs[]
@@ -2778,7 +2888,7 @@ val calls_correct = Q.store_thm("calls_correct",
     \\ IF_CASES_TAC \\ fs[] \\ strip_tac \\ rveq \\ fs[]
     \\ simp[evaluate_def]
     >- (
-      `?env5. env_rel (v_rel g1 l1) env env5 0 (MAP (λx. (0,x)) e1)` by
+      `?env5. env_rel (v_rel g1 l1 t0.code) env env5 0 (MAP (λx. (0,x)) e1)` by
           metis_tac [env_rel_env_exists]
       \\ disch_then(qspecl_then[`env5`,`t`]mp_tac)
       \\ disch_then(qspecl_then[`l1`,`g1`]mp_tac)
@@ -2787,6 +2897,12 @@ val calls_correct = Q.store_thm("calls_correct",
            (imp_res_tac evaluate_mono \\ fs[]
             \\ fs[env_rel_def,fv1_thm]
             \\ metis_tac[code_includes_SUBMAP])
+      \\ `EVERY (wfv g1 l1 t.code) env` by
+        (match_mp_tac (GEN_ALL EVERY_wfv_SUBMAP) \\ asm_exists_tac \\ fs []
+         \\ imp_res_tac evaluate_mono \\ fs [])
+      \\ `env_rel (v_rel g1 l1 t.code) env env5 0 (MAP (λx. (0,x)) e1)` by
+        (match_mp_tac (GEN_ALL env_rel_SUBMAP) \\ asm_exists_tac \\ fs []
+         \\ imp_res_tac evaluate_mono \\ fs [])
       \\ fs []
       \\ strip_tac \\ rveq
       \\ drule (Q.GEN`s`pure_correct |> INST_TYPE [``:'c``|->``:calls_state # 'c``])
@@ -2797,7 +2913,7 @@ val calls_correct = Q.store_thm("calls_correct",
       \\ ntac 2 strip_tac \\ rveq
       \\ fs[quantHeuristicsTheory.LIST_LENGTH_2] \\ rveq
       \\ rfs[] \\ rveq
-      \\ qmatch_assum_rename_tac`LIST_REL (v_rel g1 l1) ev1 ev2`
+      \\ qmatch_assum_rename_tac`LIST_REL (v_rel g1 l1 _) ev1 ev2`
       \\ Cases_on`ev1 = []`
       \\ imp_res_tac evaluate_length_imp \\ rfs[]
       \\ fs[evaluate_app_rw]
@@ -2806,8 +2922,11 @@ val calls_correct = Q.store_thm("calls_correct",
       \\ strip_tac
       \\ drule (GEN_ALL dest_closure_v_rel_lookup)
       \\ qmatch_assum_rename_tac`dest_closure _ _ f1 ev1 = _`
-      \\ rename [`v_rel g1 l1 f1 f2`]
+      \\ rename [`v_rel g1 l1 t1.code f1 f2`]
       \\ disch_then drule
+      \\ `LIST_REL (v_rel g1 l1 t1.code) ev1 ev2` by
+        (match_mp_tac (GEN_ALL LIST_REL_v_rel_SUBMAP) \\ asm_exists_tac \\ fs []
+         \\ imp_res_tac evaluate_mono \\ fs [])
       \\ disch_then drule
       \\ impl_tac >- rw[]
       \\ strip_tac
@@ -2828,6 +2947,16 @@ val calls_correct = Q.store_thm("calls_correct",
       \\ qpat_x_assum`code_includes (SND g) _`assume_tac
       \\ drule (GEN_ALL code_includes_ALOOKUP)
       \\ disch_then drule \\ strip_tac
+      \\ `t1.code = t.code` by
+       (imp_res_tac calls_sing \\ rveq \\ fs []
+        \\ drule (GEN_ALL calls_pure)
+        \\ disch_then drule \\ strip_tac
+        \\ qpat_x_assum `_ = (Rval [f2],t1)` assume_tac
+        \\ qmatch_assum_abbrev_tac `evaluate ([y],env77,t6) = _`
+        \\ drule (GEN_ALL pure_correct)
+        \\ disch_then (qspecl_then [`t6`,`env77`] mp_tac)
+        \\ fs [] \\ rw [] \\ unabbrev_all_tac \\ fs [])
+      \\ fs []
       \\ first_x_assum drule
       \\ disch_then drule
       \\ qpat_x_assum`state_rel g1 l1 r t`assume_tac
@@ -2844,10 +2973,10 @@ val calls_correct = Q.store_thm("calls_correct",
       \\ qpat_x_assum`_ = (res,_)`mp_tac
       \\ imp_res_tac state_rel_clock \\ fs[]
       \\ imp_res_tac state_rel_max_app \\ fs[]
-      \\ IF_CASES_TAC \\ fs[]
-      >- (
+      \\ IF_CASES_TAC \\ fs[] >- (
         strip_tac \\ rveq
         \\ qexists_tac`ck` \\ simp[find_code_def]
+        \\ fs [wfv_state_def]
         \\ match_mp_tac state_rel_with_clock
         \\ metis_tac[state_rel_subg] )
       \\ strip_tac
@@ -2865,8 +2994,14 @@ val calls_correct = Q.store_thm("calls_correct",
       \\ ntac 2 (qpat_x_assum`_ _ _ = (_,_)`mp_tac)
       \\ TOP_CASE_TAC \\ fs []
       \\ TOP_CASE_TAC \\ fs []
-      \\ imp_res_tac evaluate_SING \\ rveq \\ fs [])
-    \\ `env_rel (v_rel g1 l1) env env2 0 (MAP (λx. (0,x)) e1)` by fs []
+      \\ imp_res_tac evaluate_SING \\ rveq \\ fs []
+      \\ strip_tac \\ rveq \\ fs []
+      \\ imp_res_tac evaluate_mono \\ fs [] \\ rw []
+      \\ match_mp_tac (GEN_ALL wfv_state_SUBMAP) \\ asm_exists_tac \\ fs [])
+    \\ `env_rel (v_rel g1 l1 t0.code) env env2 0 (MAP (λx. (0,x)) e1)` by fs []
+    \\ `env_rel (v_rel g1 l1 t.code) env env2 0 (MAP (λx. (0,x)) e1)` by
+        (match_mp_tac (GEN_ALL env_rel_SUBMAP) \\ asm_exists_tac \\ fs []
+         \\ imp_res_tac evaluate_mono \\ fs [])
     \\ disch_then(qspecl_then[`env2`,`t`]mp_tac)
     \\ disch_then(qspecl_then[`l1`,`g1`]mp_tac)
     \\ `set (code_locs [x1]) DIFF domain (FST g) ⊆ l1` by fs [SUBSET_DEF]
@@ -2874,6 +3009,9 @@ val calls_correct = Q.store_thm("calls_correct",
          (imp_res_tac evaluate_mono \\ fs[]
           \\ fs[env_rel_def,fv1_thm]
           \\ metis_tac[code_includes_SUBMAP])
+    \\ `EVERY (wfv g1 l1 t.code) env` by
+        (match_mp_tac (GEN_ALL EVERY_wfv_SUBMAP) \\ asm_exists_tac \\ fs []
+         \\ imp_res_tac evaluate_mono \\ fs [])
     \\ fs []
     \\ strip_tac \\ rveq
     \\ strip_tac \\ rveq
@@ -2901,7 +3039,7 @@ val calls_correct = Q.store_thm("calls_correct",
     \\ rpt(disch_then drule)
     \\ simp[RIGHT_EXISTS_IMP_THM,RIGHT_EXISTS_AND_THM,FORALL_AND_THM]
     \\ strip_tac
-    \\ qmatch_assum_rename_tac`LIST_REL (v_rel g1 l1) ev1 ev2`
+    \\ qmatch_assum_rename_tac`LIST_REL (v_rel g1 l1 _) ev1 ev2`
     \\ Cases_on`ev1 = []` \\ fs[]
     \\ fs[evaluate_app_rw]
     \\ Cases_on`ev2 = []` \\ fs[]
@@ -2910,10 +3048,12 @@ val calls_correct = Q.store_thm("calls_correct",
     \\ BasicProvers.TOP_CASE_TAC \\ fs[]
     \\ drule (GEN_ALL dest_closure_v_rel_lookup)
     \\ disch_then drule
+    \\ `LIST_REL (v_rel g1 l1 t'.code) ev1 ev2` by
+        (match_mp_tac (GEN_ALL LIST_REL_v_rel_SUBMAP) \\ asm_exists_tac \\ fs []
+         \\ imp_res_tac evaluate_mono \\ fs [])
     \\ disch_then drule
     \\ impl_tac >- rw[]
     \\ strip_tac \\ fs[]
-    \\ qpat_x_assum`_ _ _ _ = (_,_)`mp_tac
     \\ imp_res_tac state_rel_clock \\ fs[]
     \\ imp_res_tac state_rel_max_app \\ fs[]
     \\ imp_res_tac LIST_REL_LENGTH \\ fs[]
@@ -2931,6 +3071,7 @@ val calls_correct = Q.store_thm("calls_correct",
       \\ rpt(first_x_assum drule)
       \\ simp[] )
     \\ strip_tac \\ rfs[]
+    \\ pop_assum mp_tac
     \\ imp_res_tac code_includes_ALOOKUP \\ fs[]
     \\ IF_CASES_TAC \\ fs[]
     >- (
@@ -2941,12 +3082,48 @@ val calls_correct = Q.store_thm("calls_correct",
       \\ imp_res_tac evaluate_mono
       \\ fs [SUBMAP_DEF,FLOOKUP_DEF]
       \\ imp_res_tac evaluate_IMP_LENGTH \\ fs []
-      \\ fs [state_rel_def])
-    \\ qpat_x_assum`_ = (_,_)`mp_tac
+      \\ fs [state_rel_def]
+      \\ match_mp_tac (GEN_ALL wfv_state_SUBMAP)
+      \\ fs [wfv_state_def]
+      \\ asm_exists_tac \\ fs [])
+    \\ `EVERY (wfv g1 l1 t'.code) ev1` by
+        (match_mp_tac (GEN_ALL EVERY_wfv_SUBMAP) \\ asm_exists_tac \\ fs []
+         \\ imp_res_tac evaluate_mono \\ fs [])
+    \\ `LIST_REL (v_rel g1 l1 t'.code) ev1 ev2` by
+        (match_mp_tac (GEN_ALL LIST_REL_v_rel_SUBMAP) \\ asm_exists_tac \\ fs []
+         \\ imp_res_tac evaluate_mono \\ fs [])
+    \\ first_x_assum drule
+    \\ disch_then drule
+    \\ disch_then drule
+    \\ strip_tac
     \\ simp[Once dec_clock_def]
     \\ simp[evaluate_def,evaluate_GENLIST_Var_tra,TAKE_APPEND1,find_code_def]
     \\ `FLOOKUP t'.code (x + 1) = FLOOKUP t.code (x + 1)` by
       (imp_res_tac evaluate_mono \\ fs [SUBMAP_DEF,FLOOKUP_DEF]) \\ fs[]
+    \\ strip_tac
+    \\ cheat (* needs updating
+    \\ asm_exists_tac \\ fs []
+    \\ goal_assum (first_x_assum o mp_then Any mp_tac)
+    \\ simp [GSYM PULL_EXISTS]
+    \\ conj_tac THEN1
+        (match_mp_tac (GEN_ALL wfv_state_SUBMAP) \\ asm_exists_tac \\ fs []
+         \\ imp_res_tac evaluate_app_mono \\ fs [])
+    \\ qpat_x_assum`evaluate(es,env2,_) = _`(mp_tac o MATCH_MP evaluate_add_clock)
+    \\ disch_then(qspec_then`ck''+ck'`mp_tac) \\ simp[] \\ strip_tac
+    \\ qexists_tac`ck+ck'+ck''` \\ simp[]
+    \\ qpat_x_assum`evaluate([_],env2,_) = _`(mp_tac o MATCH_MP evaluate_add_clock)
+    \\ disch_then(qspec_then`ck''`mp_tac) \\ simp[] \\ strip_tac
+    \\ simp_tac std_ss [GSYM APPEND_ASSOC,APPEND,TAKE_APPEND1] \\ fs []
+    \\ reverse IF_CASES_TAC \\ fs []
+    THEN1 cheat
+    \\ `FLOOKUP t'.code (x + 1) = FLOOKUP t.code (x + 1)` by
+      (imp_res_tac evaluate_mono \\ fs [SUBMAP_DEF,FLOOKUP_DEF]) \\ fs[]
+    \\ fs []
+    \\ imp_res_tac LIST_REL_LENGTH \\ fs []
+    \\ imp_res_tac evaluate_IMP_LENGTH \\ fs [] \\ rfs []
+    \\ rpt (qpat_x_assum`_ = (_,_)` (assume_tac o GSYM)) \\ fs []
+    \\ ntac 2 (TOP_CASE_TAC \\ fs [])
+    \\ drule evaluate_SING \\ strip_tac \\ fs [])
     \\ IF_CASES_TAC
     >- (
       fs[] \\ strip_tac \\ rveq \\ fs[]
@@ -2968,7 +3145,7 @@ val calls_correct = Q.store_thm("calls_correct",
     \\ simp_tac std_ss [GSYM APPEND_ASSOC,APPEND,TAKE_APPEND1] \\ fs []
     \\ rpt (qpat_x_assum`_ = (_,_)` (assume_tac o GSYM)) \\ fs []
     \\ ntac 2 (TOP_CASE_TAC \\ fs [])
-    \\ drule evaluate_SING \\ strip_tac \\ fs [])
+    \\ drule evaluate_SING \\ strip_tac \\ fs [] *))
   (* Tick *)
   \\ conj_tac >- (
     fs [evaluate_def,calls_def] \\ rpt strip_tac
@@ -2982,6 +3159,8 @@ val calls_correct = Q.store_thm("calls_correct",
     \\ pairarg_tac \\ fs [] \\ rw []
     \\ fs [dec_clock_def]
     \\ first_x_assum drule \\ fs [code_locs_def]
+    \\ disch_then (qspecl_then [`env2`,`dec_clock 1 t0`] mp_tac)
+    \\ fs [dec_clock_def]
     \\ rpt (disch_then drule) \\ fs []
     \\ fs [GSYM PULL_FORALL,GSYM AND_IMP_INTRO]
     \\ impl_tac THEN1 fs [wfv_state_def]
@@ -2989,7 +3168,6 @@ val calls_correct = Q.store_thm("calls_correct",
     \\ `includes_state g1 s.compile_oracle` by
           (imp_res_tac evaluate_includes_state \\ fs [])
     \\ fs [PULL_FORALL,AND_IMP_INTRO]
-    \\ disch_then (qspecl_then [`env2`,`t0 with clock := t0.clock-1`] mp_tac)
     \\ impl_tac THEN1 (fs [state_rel_def,env_rel_def,fv1_thm] \\ rfs []
                        \\ imp_res_tac calls_sing \\ fs [])
     \\ strip_tac \\ fs []
@@ -3002,6 +3180,7 @@ val calls_correct = Q.store_thm("calls_correct",
     \\ qpat_x_assum `_ = (_,_)` mp_tac
     \\ pop_assum (fn th => simp_tac std_ss [th])
     \\ fs [])
+
   (* Call *)
   \\ conj_tac >- (
     rw[evaluate_def,calls_def,code_locs_def,ALL_DISTINCT_APPEND]
@@ -3031,6 +3210,7 @@ val calls_correct = Q.store_thm("calls_correct",
     \\ qexists_tac `ck` \\ fs [evaluate_def])
   \\ conj_tac >- ( rw[evaluate_def] \\ qexists_tac`0`
                    \\ rw[RIGHT_EXISTS_IMP_THM,RIGHT_EXISTS_AND_THM] )
+
   (* app cons *)
   \\ simp[evaluate_def]
   \\ rpt gen_tac \\ strip_tac
@@ -3039,15 +3219,17 @@ val calls_correct = Q.store_thm("calls_correct",
   >- (
     simp[PULL_EXISTS]
     \\ rpt gen_tac \\ strip_tac
+    \\ qabbrev_tac `t1 = if s0.clock < SUC (LENGTH v69) then t0 with clock := 0
+                         else dec_clock (SUC (LENGTH v69)) t0`
+    \\ `every_result (EVERY (wfv g l t1.code)) (wfv g l t1.code) res` by (
+      every_case_tac \\ fs[] \\ rveq \\ fs[Abbr`t1`,dec_clock_def]
+      \\ match_mp_tac (GEN_ALL dest_closure_partial_wfv)
+      \\ asm_exists_tac \\ fs[] )
+    \\ asm_exists_tac \\ fs []
     \\ simp[RIGHT_EXISTS_AND_THM,RIGHT_EXISTS_IMP_THM]
     \\ conj_asm1_tac
     >- (
-      every_case_tac \\ fs[] \\ rveq \\ fs[]
-      \\ match_mp_tac (GEN_ALL dest_closure_partial_wfv)
-      \\ asm_exists_tac \\ fs[] )
-    \\ conj_asm1_tac
-    >- (
-      every_case_tac \\ fs[] \\ rveq \\ fs[]
+      every_case_tac \\ fs[Abbr`t1`] \\ rveq \\ fs[]
       \\ fs[wfv_state_def,dec_clock_def] )
     \\ simp[evaluate_app_rw]
     \\ drule (GEN_ALL dest_closure_v_rel)
@@ -3058,7 +3240,7 @@ val calls_correct = Q.store_thm("calls_correct",
     \\ imp_res_tac state_rel_max_app \\ fs[]
     \\ qexists_tac`0` \\ fs[]
     \\ imp_res_tac LIST_REL_LENGTH
-    \\ rw[] \\ fs[] \\ rw[dec_clock_def]
+    \\ rw[] \\ fs[] \\ rw[dec_clock_def] \\ fs [Abbr`t1`,dec_clock_def]
     \\ match_mp_tac state_rel_with_clock \\ fs[] )
   \\ fs[PULL_EXISTS]
   \\ rpt gen_tac \\ strip_tac
@@ -3067,8 +3249,10 @@ val calls_correct = Q.store_thm("calls_correct",
   \\ IF_CASES_TAC
   >- (
     simp[] \\ strip_tac \\ rveq \\ fs[]
-    \\ conj_tac >- fs[wfv_state_def]
+    \\ simp[RIGHT_EXISTS_AND_THM,RIGHT_EXISTS_IMP_THM]
     \\ qexists_tac`0` \\ fs[]
+    \\ qexists_tac`t0 with clock := 0` \\ fs[]
+    \\ conj_tac >- fs[wfv_state_def]
     \\ simp[RIGHT_EXISTS_AND_THM,RIGHT_EXISTS_IMP_THM]
     \\ rw[evaluate_app_rw]
     \\ drule (GEN_ALL dest_closure_v_rel)
@@ -3088,10 +3272,8 @@ val calls_correct = Q.store_thm("calls_correct",
       \\ imp_res_tac evaluate_includes_state
       \\ imp_res_tac evaluate_app_includes_state
       \\ fs [dec_clock_def])
-  \\ qmatch_abbrev_tac`c1 ∧ c2 ∧ _`
   \\ qmatch_asmsub_rename_tac`wfv g1 l1`
   \\ qmatch_asmsub_rename_tac`Full_app e args rest`
-  \\ fs[Abbr`c1`,Abbr`c2`]
   \\ simp[RIGHT_EXISTS_AND_THM,RIGHT_EXISTS_IMP_THM]
   \\ drule (GEN_ALL dest_closure_v_rel) \\ fs[PULL_EXISTS]
   \\ rpt (disch_then drule)
@@ -3107,11 +3289,11 @@ val calls_correct = Q.store_thm("calls_correct",
   \\ fs[PULL_EXISTS] \\ rfs[]
   \\ fs[recclosure_rel_def]
   \\ rpt(pairarg_tac \\ fs[])
-  \\ qmatch_assum_rename_tac`v_rel g1 l1 f f'`
+  \\ qmatch_assum_rename_tac`v_rel g1 l1 _ f f'`
   \\ qmatch_assum_rename_tac`LIST_REL _ rest1 rest2`
   \\ first_x_assum(qspecl_then[`g1`,`l1`]mp_tac o
         CONV_RULE(RESORT_FORALL_CONV List.rev))
-  \\ `EVERY (wfv g1 l1) args /\ EVERY (wfv g1 l1) rest1` by
+  \\ `EVERY (wfv g1 l1 t0.code) args /\ EVERY (wfv g1 l1 t0.code) rest1` by
    (last_assum (mp_then (Pos hd) mp_tac (GEN_ALL dest_closure_full_wfv))
     \\ disch_then drule \\ impl_tac THEN1 fs [] \\ rw [] \\ fs [])
   \\ ((fn g as (asl,w) =>
@@ -3138,7 +3320,7 @@ val calls_correct = Q.store_thm("calls_correct",
   \\ qmatch_asmsub_abbrev_tac`COND b`
   \\ rveq \\ fs []
   \\ imp_res_tac calls_length \\ fs[]
-  \\ `env_rel (v_rel g1 l1) args args2 0 [(0, SND (EL i fns2))]`
+  \\ `env_rel (v_rel g1 l1 t0.code) args args2 0 [(0, SND (EL i fns2))]`
   by (
     qhdtm_x_assum`env_rel`mp_tac
     \\ `n = FST (EL i fns2)`
@@ -3163,9 +3345,7 @@ val calls_correct = Q.store_thm("calls_correct",
     \\ simp[] \\ fs[]
     \\ fs[LIST_REL_EL_EQN]
     \\ rfs[EL_TAKE])
-
   \\ (reverse(Cases_on`b`) \\ fs[] \\ rveq >- (
-
     rveq \\ drule (GEN_ALL calls_el_sing)
     \\ disch_then (qspec_then`i`mp_tac)
     \\ impl_tac >- fs[wfg_def,recclosure_wf_def]
@@ -3176,13 +3356,13 @@ val calls_correct = Q.store_thm("calls_correct",
     \\ impl_tac
     >- (
       fs[dec_clock_def]
+      \\ conj_tac >- fs [wfv_state_def]
       \\ conj_tac >- metis_tac[subg_trans]
       \\ conj_tac >- fs[SUBSET_DEF]
-      \\ qhdtm_x_assum`env_rel`mp_tac
-      \\ simp[EL_ZIP]
-      \\ rw []
+      \\ qhdtm_x_assum`env_rel`mp_tac \\ simp[EL_ZIP] \\ rw []
       THEN1 metis_tac[state_rel_with_clock,code_includes_subg,state_rel_def]
-      \\ cheat)
+      \\ match_mp_tac (MP_CANON (GEN_ALL code_includes_subg))
+      \\ asm_exists_tac \\ fs [])
     \\ strip_tac
     \\ imp_res_tac calls_length \\ fs[]
     \\ simp[EL_ZIP]
@@ -3193,6 +3373,15 @@ val calls_correct = Q.store_thm("calls_correct",
     \\ rfs[EL_ZIP]
     \\ TRY (qexists_tac`ck` \\ simp[] \\ rfs[] \\ NO_TAC)
     \\ first_x_assum drule
+    \\ `EVERY (wfv g1 l1 t.code) rest1` by
+      (match_mp_tac (GEN_ALL EVERY_wfv_SUBMAP) \\ asm_exists_tac
+       \\ imp_res_tac evaluate_mono \\ fs [])
+    \\ `wfv_state g1 l1 t.code r` by
+      (match_mp_tac (GEN_ALL wfv_state_SUBMAP) \\ asm_exists_tac
+       \\ imp_res_tac evaluate_mono \\ fs [])
+    \\ `LIST_REL (v_rel g1 l1 t.code) rest1 rest2` by
+      (match_mp_tac (GEN_ALL LIST_REL_v_rel_SUBMAP) \\ asm_exists_tac
+       \\ imp_res_tac evaluate_mono \\ fs [])
     \\ rpt (disch_then (first_assum o mp_then Any mp_tac))
     \\ rw [] \\ fs []
     \\ rpt (goal_assum (first_assum o mp_then Any mp_tac)) \\ fs []
@@ -3211,9 +3400,7 @@ val calls_correct = Q.store_thm("calls_correct",
     \\ IF_CASES_TAC \\ fs[] )
   \\ simp[EVAL``(closSem$dec_clock _ _).code``]
   \\ qmatch_assum_abbrev_tac`subg gd g1`
-
-  \\ `code_includes (SND gd) t0.code`
-  by cheat
+  \\ qpat_x_assum `code_includes (SND gd) t0.code` assume_tac
   \\ pop_assum mp_tac
   \\ `ALOOKUP (SND gd) (2 * i + loc + 1) = SOME (EL i (ZIP (MAP FST fns1,es)))`
   by (
@@ -3268,6 +3455,7 @@ val calls_correct = Q.store_thm("calls_correct",
   \\ disch_then(qspecl_then[`dec_clock dk t0`,`TAKE n args2`]mp_tac)
   \\ (impl_tac >- (
     fs[dec_clock_def]
+    \\ conj_tac >- fs [wfv_state_def]
     \\ conj_tac >- (
       match_mp_tac subg_trans \\ asm_exists_tac \\ fs []
       \\ match_mp_tac subg_trans \\ once_rewrite_tac [CONJ_COMM]
@@ -3386,6 +3574,12 @@ val calls_correct = Q.store_thm("calls_correct",
           \\ `ck + (t0.clock − dk) = ck + t0.clock − dk` by decide_tac
           \\ fs [] \\ NO_TAC)
   \\ first_x_assum drule
+  \\ `EVERY (wfv g1 l1 t.code) rest1` by
+    (match_mp_tac (GEN_ALL EVERY_wfv_SUBMAP) \\ asm_exists_tac \\ fs []
+     \\ imp_res_tac evaluate_mono \\ fs [])
+  \\ `LIST_REL (v_rel g1 l1 t.code) rest1 rest2` by
+    (match_mp_tac (GEN_ALL LIST_REL_v_rel_SUBMAP) \\ asm_exists_tac \\ fs []
+     \\ imp_res_tac evaluate_mono \\ fs [])
   \\ rpt (disch_then drule) \\ fs []
   \\ rw [] \\ fs [ADD1]
   \\ rpt (goal_assum (first_x_assum o mp_then Any mp_tac))
